src/LibOtherDemos.v
@@ -5,65 +5,48 @@
 
 Set Implicit Arguments.
 Require Import LibTactics.
-
-Require LibLogic LibList LibRelation LibWf LibList LibLN.
-
-
-
+Require Import LibLogic LibEqual LibList LibRelation LibWf LibList LibLN.
 
 
 (* ---------------------------------------------------------------------- *)
 (** ** Demo of extens tactics *)
 
-Lemma test : forall A1 (P Q :  A1->Prop),
+Lemma test_extensionality_1 : forall A1 (P Q :  A1->Prop),
   (forall x1, P x1 <-> Q x1) -> 
   P = Q.
 Proof using. 
-
   intros. applys extensionality. hnf.
 Abort.
   
-Lemma prop_ext_2' : forall A1 (A2: A1->Type) (P Q : forall (x1:A1) (x2:A2 x1), Prop),
+Lemma test_extensionality_2 : forall A1 (A2: A1->Type) (P Q : forall (x1:A1) (x2:A2 x1), Prop),
   (forall x1 x2, P x1 x2 <-> Q x1 x2) -> 
   P = Q.
   intros. applys extensionality. hnf.
 Abort.
-
-
-Lemma test : forall A1 (P Q : forall (x1:A1), Prop),
-  (forall x1, P x1 <-> Q x1) -> 
-  P = Q.
-Proof using. 
-
-  intros. applys extensionality. hnf.
-  
 
 Section FuncExtDepTest.
 Variables (A1 : Type).
 Variables (A2 : forall (x1 : A1), Type).
 Variables (A3 : forall (x1 : A1) (x2 : A2 x1), Type).
 Variables (A4 : forall (x1 : A1) (x2 : A2 x1) (x3 : A3 x2), Type).
+
 Lemma test_fun_ext_3 : forall (f g : forall (x1:A1) (x2:A2 x1) (x3:A3 x2), A4 x3),
   (forall x1 x2 x3, f x1 x2 x3 = g x1 x2 x3) -> 
   f = g.
-Proof using. intros. applys extensionality. hnf. Qed.
+Proof using. intros. applys extensionality. hnf. Abort.
+
 End FuncExtDepTest.
-
-
 
 Lemma prop_ext_1_test : forall (P Q : Prop),
   (P <-> Q) -> 
   P = Q.
-Proof using. intros. applys extensionality. simpl extensionality_hyp. Abort.
- extens*. 
-
-
+Proof using. 
+  intros. applys extensionality. simpl extensionality_hyp. 
+Abort.
 
 
 (* ---------------------------------------------------------------------- *)
 (** ** Demo of LibLogic tactics *)
-
-
 Lemma absurds_demo : forall (P Q : Prop),  
   P /\ (~ P) /\ (Q \/ ~ P).
 Proof using.
@@ -72,7 +55,6 @@ Proof using.
   { absurds ;=> H. admit. }
   { absurds ;=> (H1&H2). admit. }
 Abort.
-
 
 
 (* ********************************************************************** *)
@@ -201,15 +183,15 @@ Qed.
 Lemma tree_induct_mem : forall (P : tree -> Prop),
   (forall n : nat, P (leaf n)) ->
   (forall ts : list tree,
-    (forall t, Mem t ts -> P t) -> P (node ts)) ->
+    (forall t, mem t ts -> P t) -> P (node ts)) ->
   forall t : tree, P t.
 Proof using.
   introv Hl Hn. eapply tree_induct_gen with (Q := fun ts =>
-    forall t, Mem t ts -> P t); intros.
+    forall t, mem t ts -> P t); intros.
   auto. auto. inverts H. inverts~ H1.
 Qed.
 
-Hint Constructors Mem.
+Hint Constructors mem.
 
 (** Example of an inductive proof with Mem
     -- usually not as good as the one with [Forall] *)
@@ -232,7 +214,7 @@ Import LibRelation LibWf.
 
 Inductive subtree : binary tree :=
   | subtree_intro : forall t ts,
-     Mem t ts -> subtree t (node ts).
+     mem t ts -> subtree t (node ts).
   (* there is typically more than one case here *)
 
 Hint Constructors subtree.
